Proving the correctness of the map template

Compiler/CUDALib.v
@@ -108,11 +108,11 @@ Fixpoint maptys {ty T1 T2} (f : T1 -> T2) :=
     (maptys f (fst xs), maptys f (snd xs))
   end.
 
-Definition v2e {ty} := @maptys ty _ _ Evar.
-Definition e2sh {ty} := @maptys ty _ _ Sh.
-Definition e2gl {ty} := @maptys ty _ _ Gl.
-Definition v2sh {ty} (xs : vars ty) := (e2sh (v2e xs)).
-Definition v2gl {ty} (xs : vars ty) := (e2gl (v2e xs)).
+Definition v2e {ty} : vars ty -> exps ty := @maptys ty _ _ Evar.
+Definition e2sh {ty} : exps ty -> lexps ty := @maptys ty _ _ Sh.
+Definition e2gl {ty} : exps ty -> lexps ty := @maptys ty _ _ Gl.
+Definition v2sh {ty} (xs : vars ty) : lexps ty := (e2sh (v2e xs)).
+Definition v2gl {ty} (xs : vars ty) : lexps ty := (e2gl (v2e xs)).
 
 Fixpoint ty2ctys ty :=
   match ty return ctys ty with
